\documentclass{article}

\usepackage{units}
\usepackage{booktabs}
\usepackage{graphicx}
\usepackage{amsmath, amsthm, amssymb, bm}
\usepackage{tikz, pgfplots}
\usepackage{lipsum}
\usepackage{mwe}
\usetikzlibrary{shapes, arrows, positioning, fit, calc}
\newtheorem{theorem}{Theorem}
\newtheorem{Property}{Property}
\theoremstyle{remark}
\newtheorem*{defn}{Definition}
\renewcommand{\vec}[1]{\underline{#1}}
\usepackage{units}
\usepackage{fancyvrb}
\usepackage{hyperref}
\fvset{fontsize=\normalsize}

\title{AI1103 Assignement 2}
\author{Hritik Sarkar}

\newcommand\numberthis{\addtocounter{equation}{1}\tag{\theequation}}
\newcommand\inv[1]{#1\raisebox{1.15ex}{$\scriptscriptstyle-\!1$}}

\begin{document}

\maketitle
Paper - \href{https://github.com/gadepall/papers/blob/master/ugc/math/2019.pdf}{UGC 2019}
\newline
\\ Q59. Suppose that $\begin{pmatrix} X\\ Y \end{pmatrix}$ has a bivariate density $f = \frac{1}{2}f_1 + \frac{1}{2}f_2$, where $f_1$ and $f_2$ are respectively, the densities of bivariate normal distribution $N(\mu_{1},\sum)$, and $N(\mu_{2},\sum)$, with $\mu_{1} = \begin{pmatrix} 1 \\ 1 \end{pmatrix}$, $\mu_{2} = \begin{pmatrix} -1 \\ -1 \end{pmatrix}$ and $\sum = \mathbb{I}_{2}$, the $2 \times 2$ identity matrix. Then which of the following is correct ?
\newline
\\a) $X$ and $Y$ are positively correlated
\\b) $X$ and $Y$ are negatively correlated
\\c) $X$ and $Y$ are uncorrelated but they are not independent
\\d) $X$ and $Y$ are independent
\newline
\\ Answer:
\newline

To check the correlation between $X$ and $Y$ we can calculate the covariance of $X$ and $Y$. If the value of covariance is $+ve$ then $ X$ and $Y$ are positively correlated, if the value is $-ve$ then $X$ and $Y$ are negatively correlated and if the value is 0 then $X$ and $Y$ are independent.\\
\newline
For a bivariate, covariance is defind as \\
\[ cov(X,Y) = \int_{-\infty}^{\infty} \int_{-\infty}^{\infty} (x-\mu_{x}) (y-\mu{y}) f(x,y) dx dy \numberthis \label{-1}\]
The bivariate normal distribution is defined as 
\[
f(\vec{X}) = \left ( 2\pi\sqrt{\left | \sum \right |} \right )^{-1} e^{-\frac{1}{2}[(\vec{X}-\vec{\mu})^T\sum^{-1}(\vec{X}-\vec{\mu})]} \numberthis \label{0}\]
where
\[ 
\vec{X} = \begin{pmatrix}
X\\ 
Y
\end{pmatrix}, 
\sum =  \begin{pmatrix}
 Var[X]& Cov(X,Y)\\ 
 Cov(X,Y)& Var[Y] 
\end{pmatrix} = \begin{pmatrix}
\sigma_X^2  & \rho \sigma_X \sigma_Y\\ 
\rho \sigma_X \sigma_Y & \sigma_Y^2
\end{pmatrix}
\]
$\rho$ is the correlation coefficient.\\
\newline
The mean can be obtained as such
\[ \mathop{\mathbb{E}}\left[\begin{pmatrix} X\\ Y \end{pmatrix} \right ]= \frac{1}{2} \mu_{1} + \frac{1}{2} \mu_{2} = \begin{pmatrix} 0\\0 \end{pmatrix}\]
and 
\[
    \sum = \mathbb{I}_2
\]
so, \[\left | \sum \right | = 1\], \[ \inv{\sum} = \mathbb{I}_2 \]
Now,
\begin{align*}
    Cov(X,Y) &=  \int_{-\infty}^{\infty} \int_{-\infty}^{\infty} x y (\frac{1}{2}f_1+\frac{1}{2}f_2) dx dy \\
    &= \frac{1}{2} \int_{-\infty}^{\infty} \int_{-\infty}^{\infty} x y f_1 dx dy + \frac{1}{2} \int_{-\infty}^{\infty} \int_{-\infty}^{\infty} x y f_2 dx dy \numberthis \label{1}\\
\end{align*}
consider,
\begin{align*}
    I_1 &= \frac{1}{2} \int_{-\infty}^{\infty} \int_{-\infty}^{\infty} x y f_1 dx dy \\
    &= \frac{1}{2} \int_{-\infty}^{\infty} \int_{-\infty}^{\infty} x y \frac{1}{2\pi} e^{-\frac{1}{2}[(\vec{X}-\vec{\mu_1})^T(\vec{X}-\vec{\mu_1})]} dx dy \\
    &= \frac{1}{4\pi} \int_{-\infty}^{\infty} \int_{-\infty}^{\infty} x y e^{-\frac{1}{2}\left ( \left \| \vec{X} \right \|^2 + \left \| \vec{\mu_1} \right \|^2 -2 \vec{X}^T\vec{\mu_1} \right )} dx dy\\
    &= \frac{1}{4\pi} \int_{-\infty}^{\infty} \int_{-\infty}^{\infty} xye^{-\frac{1}{2}(x^2+y^2+2-2x-2y)} dx dy \\
    &= \frac{1}{4\pi} \int_{-\infty}^{\infty} x e^{-\frac{1}{2}(x-1)^2} dx \int_{-\infty}^{\infty} y e^{-\frac{1}{2}(y-1)^2}  dy \numberthis \label{2}\\
\end{align*}
let,
\begin{align*}
    I_2 &= \int_{-\infty}^{\infty} x e^{-\frac{1}{2}(x-1)^2}\\
\end{align*}
observe,
\begin{align*}
    \int_{-\infty}^{\infty} e^{-\frac{1}{2}(x-1)^2} dx - I_2 &= \int_{-\infty}^{\infty} (1-x) e^{-\frac{1}{2}(x-1)^2} dx\\
    &= \int_{-\infty}^{\infty} \frac{\mathrm{d}}{\mathrm{d} x}\left ( e^{-\frac{1}{2}(x-1)^2} \right ) dx \\
    &= \left [   e^{-\frac{1}{2}(x-1)^2} \right ]_{-\infty}^{\infty} \\
    &= 0 \numberthis \label{3}
\end{align*}
So from \eqref{3},
\begin{align*}
   I_2 &=  \int_{-\infty}^{\infty} e^{-\frac{1}{2}(x-1)^2} dx\\
   &= \int_{-\infty}^{\infty} e^{-\frac{1}{2}u^2} du &\textit{($u=x-1)$}
\end{align*}
now,
\begin{align*}
    I_2^2 &= \int_{-\infty}^{\infty} e^{-\frac{1}{2}u^2} du \int_{-\infty}^{\infty} e^{-\frac{1}{2}v^2} dv &\textit{($v$ is a dummy variable)}
    \\&= \int_{-\infty}^{\infty} \int_{-\infty}^{\infty} e^{-\frac{1}{2}(u^2+v^2)} du dv
    \\&=\int_{0}^{\infty} \int_{0}^{2\pi} e^{-\frac{1}{2}r^2} r dr d\theta &\textit{\href{https://www.youtube.com/watch?v=fWOGfzC3IeY}{(changing to polar co-ordinates)}}\\
    &= 2\pi \numberthis \label{4}
\end{align*}
So from \eqref{4},
\begin{align*}
    I_2 = \sqrt(2\pi)
\end{align*}
Now going back to \eqref{2},
\begin{align*}
    I_1 &= \frac{1}{4\pi}*\sqrt(2\pi)*\sqrt(2\pi) &\textit{(integral over $y$ is exactly same)}\\
    &= \frac{1}{2}
\end{align*}
Now from \eqref{1},
\begin{align*}
    Cov(X,Y) &= \frac{1}{2} + \frac{1}{2} &\textit{(second part is similar)}\\
    &=1
\end{align*}
Since $Cov(X,Y)$ is $+ve$, $X$ and $Y$ are positively correlated. (Ans.)
\end{document}